specs/L1AssetRouter/L1AssetRouter/Common/switch_8800258257933484115_user.lean
@@ -13,12 +13,14 @@ section
 
 open Clear EVMState Ast Expr Stmt FunctionDefinition State Interpreter ExecLemmas OutOfFuelLemmas Abstraction YulNotation PrimOps ReasoningPrinciple Utilities generated.L1AssetRouter L1AssetRouter
 
-def A_switch_8800258257933484115 (s₀ s₉ : State) : Prop := sorry
+def A_switch_8800258257933484115 (s₀ s₉ : State) : Prop :=
+  switch_8800258257933484115_concrete_of_code.1 s₀ s₉
 
 lemma switch_8800258257933484115_abs_of_concrete {s₀ s₉ : State} :
   Spec switch_8800258257933484115_concrete_of_code s₀ s₉ →
   Spec A_switch_8800258257933484115 s₀ s₉ := by
-  sorry
+  unfold A_switch_8800258257933484115
+  simpa [switch_8800258257933484115_concrete_of_code]
 
 end
 
