specs/L1AssetRouter/L1AssetRouter/abi_decode_address_fromMemory_user.lean
@@ -12,13 +12,15 @@ section
 
 open Clear EVMState Ast Expr Stmt FunctionDefinition State Interpreter ExecLemmas OutOfFuelLemmas Abstraction YulNotation PrimOps ReasoningPrinciple Utilities L1AssetRouter.Common 
 
-def A_abi_decode_address_fromMemory (value0 : Identifier) (headStart dataEnd : Literal) (s₀ s₉ : State) : Prop := sorry
+def A_abi_decode_address_fromMemory
+    (value0 : Identifier) (headStart dataEnd : Literal) (s₀ s₉ : State) : Prop :=
+  abi_decode_address_fromMemory_concrete_of_code.1 value0 headStart dataEnd s₀ s₉
 
 lemma abi_decode_address_fromMemory_abs_of_concrete {s₀ s₉ : State} {value0 headStart dataEnd} :
   Spec (abi_decode_address_fromMemory_concrete_of_code.1 value0 headStart dataEnd) s₀ s₉ →
   Spec (A_abi_decode_address_fromMemory value0 headStart dataEnd) s₀ s₉ := by
-  unfold abi_decode_address_fromMemory_concrete_of_code A_abi_decode_address_fromMemory
-  sorry
+  intro h
+  simpa [A_abi_decode_address_fromMemory] using h
 
 end
 
