specs/L1AssetRouter/L1AssetRouter/abi_decode_address_payable_fromMemory_user.lean
@@ -11,13 +11,15 @@ section
 
 open Clear EVMState Ast Expr Stmt FunctionDefinition State Interpreter ExecLemmas OutOfFuelLemmas Abstraction YulNotation PrimOps ReasoningPrinciple Utilities L1AssetRouter.Common 
 
-def A_abi_decode_address_payable_fromMemory (value : Identifier) (offset : Literal) (s₀ s₉ : State) : Prop := sorry
+def A_abi_decode_address_payable_fromMemory
+    (value : Identifier) (offset : Literal) (s₀ s₉ : State) : Prop :=
+  abi_decode_address_payable_fromMemory_concrete_of_code.1 value offset s₀ s₉
 
 lemma abi_decode_address_payable_fromMemory_abs_of_concrete {s₀ s₉ : State} {value offset} :
   Spec (abi_decode_address_payable_fromMemory_concrete_of_code.1 value offset) s₀ s₉ →
   Spec (A_abi_decode_address_payable_fromMemory value offset) s₀ s₉ := by
-  unfold abi_decode_address_payable_fromMemory_concrete_of_code A_abi_decode_address_payable_fromMemory
-  sorry
+  intro h
+  simpa [A_abi_decode_address_payable_fromMemory] using h
 
 end
 
