specs/L1AssetRouter/L1AssetRouter/allocate_and_zero_memory_array_array_bytes_dyn_user.lean
@@ -1,8 +1,9 @@
 import Clear.ReasoningPrinciple
 
-import generated.L1AssetRouter.L1AssetRouter.Common.if_9161423447775431245
+import generated.L1AssetRouter.L1AssetRouter.Common.if_5742678230396989370
 import generated.L1AssetRouter.L1AssetRouter.finalize_allocation
-import generated.L1AssetRouter.L1AssetRouter.Common.for_834482124796821278
+import generated.L1AssetRouter.L1AssetRouter.Common.if_6292600599473441644
+import generated.L1AssetRouter.L1AssetRouter.Common.for_5632825108664701324
 
 import generated.L1AssetRouter.L1AssetRouter.allocate_and_zero_memory_array_array_bytes_dyn_gen
 
@@ -13,13 +14,14 @@ section
 
 open Clear EVMState Ast Expr Stmt FunctionDefinition State Interpreter ExecLemmas OutOfFuelLemmas Abstraction YulNotation PrimOps ReasoningPrinciple Utilities L1AssetRouter.Common generated.L1AssetRouter L1AssetRouter
 
-def A_allocate_and_zero_memory_array_array_bytes_dyn (memPtr : Identifier)  (s₀ s₉ : State) : Prop := sorry
+def A_allocate_and_zero_memory_array_array_bytes_dyn (memPtr : Identifier)  (s₀ s₉ : State) : Prop :=
+  allocate_and_zero_memory_array_array_bytes_dyn_concrete_of_code.1 memPtr s₀ s₉
 
 lemma allocate_and_zero_memory_array_array_bytes_dyn_abs_of_concrete {s₀ s₉ : State} {memPtr } :
   Spec (allocate_and_zero_memory_array_array_bytes_dyn_concrete_of_code.1 memPtr ) s₀ s₉ →
   Spec (A_allocate_and_zero_memory_array_array_bytes_dyn memPtr ) s₀ s₉ := by
-  unfold allocate_and_zero_memory_array_array_bytes_dyn_concrete_of_code A_allocate_and_zero_memory_array_array_bytes_dyn
-  sorry
+  intro h
+  simpa [A_allocate_and_zero_memory_array_array_bytes_dyn] using h
 
 end
 
