specs/L1AssetRouter/L1AssetRouter/finalize_allocation_27947_user.lean
@@ -1,6 +1,6 @@
 import Clear.ReasoningPrinciple
 
-import generated.L1AssetRouter.L1AssetRouter.Common.if_5531105932464825883
+import generated.L1AssetRouter.L1AssetRouter.Common.if_6800231307417003598
 
 import generated.L1AssetRouter.L1AssetRouter.finalize_allocation_27947_gen
 
@@ -11,13 +11,14 @@ section
 
 open Clear EVMState Ast Expr Stmt FunctionDefinition State Interpreter ExecLemmas OutOfFuelLemmas Abstraction YulNotation PrimOps ReasoningPrinciple Utilities L1AssetRouter.Common 
 
-def A_finalize_allocation_27947  (memPtr : Literal) (s₀ s₉ : State) : Prop := sorry
+def A_finalize_allocation_27947  (memPtr : Literal) (s₀ s₉ : State) : Prop :=
+  finalize_allocation_27947_concrete_of_code.1 memPtr s₀ s₉
 
 lemma finalize_allocation_27947_abs_of_concrete {s₀ s₉ : State} { memPtr} :
   Spec (finalize_allocation_27947_concrete_of_code.1  memPtr) s₀ s₉ →
   Spec (A_finalize_allocation_27947  memPtr) s₀ s₉ := by
-  unfold finalize_allocation_27947_concrete_of_code A_finalize_allocation_27947
-  sorry
+  intro h
+  simpa [A_finalize_allocation_27947] using h
 
 end
 
