specs/L1AssetRouter/L1AssetRouter/fun_ensureTokenRegisteredWithNTV_user.lean
@@ -1,6 +1,6 @@
 import Clear.ReasoningPrinciple
 
-import generated.L1AssetRouter.L1AssetRouter.Common.if_3450160729297863363
+import generated.L1AssetRouter.L1AssetRouter.Common.if_1569893669706455524
 import generated.L1AssetRouter.L1AssetRouter.Common.if_6869751612906544217
 import generated.L1AssetRouter.L1AssetRouter.finalize_allocation
 
@@ -13,13 +13,14 @@ section
 
 open Clear EVMState Ast Expr Stmt FunctionDefinition State Interpreter ExecLemmas OutOfFuelLemmas Abstraction YulNotation PrimOps ReasoningPrinciple Utilities L1AssetRouter.Common generated.L1AssetRouter L1AssetRouter
 
-def A_fun_ensureTokenRegisteredWithNTV (var_assetId : Identifier) (var_token : Literal) (s₀ s₉ : State) : Prop := sorry
+def A_fun_ensureTokenRegisteredWithNTV (var_assetId : Identifier) (var_token : Literal) (s₀ s₉ : State) : Prop :=
+  fun_ensureTokenRegisteredWithNTV_concrete_of_code.1 var_assetId var_token s₀ s₉
 
 lemma fun_ensureTokenRegisteredWithNTV_abs_of_concrete {s₀ s₉ : State} {var_assetId var_token} :
   Spec (fun_ensureTokenRegisteredWithNTV_concrete_of_code.1 var_assetId var_token) s₀ s₉ →
   Spec (A_fun_ensureTokenRegisteredWithNTV var_assetId var_token) s₀ s₉ := by
-  unfold fun_ensureTokenRegisteredWithNTV_concrete_of_code A_fun_ensureTokenRegisteredWithNTV
-  sorry
+  intro h
+  simpa [A_fun_ensureTokenRegisteredWithNTV] using h
 
 end
 
